theories/interop/wp_prims/length.v
@@ -1,0 +1,51 @@
+From iris.proofmode Require Import proofmode.
+From transfinite.base_logic.lib Require Import ghost_map ghost_var.
+From melocoton Require Import named_props stdpp_extra.
+From melocoton.mlanguage Require Import mlanguage.
+From melocoton.c_interface Require Import defs notation resources.
+From melocoton.interop Require Import state lang basics_resources.
+From melocoton.interop Require Export prims weakestpre prims_proto.
+From melocoton.interop.wp_prims Require Import common.
+From melocoton.mlanguage Require Import weakestpre.
+Import Wrap.
+
+Section Laws.
+
+Context `{SI: indexT}.
+Context {Σ : gFunctors}.
+Context `{!heapG_ML Σ, !heapG_C Σ}.
+Context `{!invG Σ}.
+Context `{!wrapperG Σ}.
+
+Implicit Types P : iProp Σ.
+Import mlanguage.
+
+Lemma length_correct E e : |- prims_prog e @ E :: length_proto.
+Proof using.
+  iIntros (? ? ? ?) "H". unfold mprogwp. iNamed "H".
+  destruct bl as [tg vs0].
+  do 2 (iExists _; iSplit; first done). iNext.
+  rewrite weakestpre.wp_unfold. rewrite /weakestpre.wp_pre.
+  iIntros "Hb %σ Hσ". cbn -[prims_prog].
+  SI_at_boundary. iNamed "HGC". SI_GC_agree.
+  iDestruct "Hpto" as "(Hpto & Hptoacc)".
+  iPoseProof (lstore_own_elem_of with "GCζvirt Hpto") as "%Helem".
+  iAssert ⌜∃ m', ζC ρc !! γ = Some (Bvblock (m', (tg, vs0)))⌝%I as "%Helem2".
+  1: { iPureIntro. eapply lookup_union_Some_r in Helem; last apply Hfreezedj.
+       eapply freeze_lstore_lookup_backwards in Helem as (?&Hfrz&?); eauto.
+       inversion Hfrz; simplify_eq; eauto. }
+  destruct Helem2 as [m' Helem2].
+
+  iApply wp_pre_cases_c_prim; [done..|].
+  iExists (λ '(e', σ'), e' = WrSE (ExprV #(length vs0)) ∧ σ' = CState ρc mem).
+  iSplit. { iPureIntro; econstructor; eauto. }
+  iIntros (? ? ? (? & ?)); simplify_eq.
+  do 3 iModIntro. iFrame. iSplitL "SIinit". { iExists false. iFrame. }
+  iApply wp_value; first done.
+  iApply ("Cont" with "[-Hpto Hptoacc] [$Hpto $Hptoacc]"); try done; [].
+  rewrite /GC /named.
+  iExists _, (ζσ ∪ ζvirt), ζσ, ζvirt, _, χvirt, σMLvirt, _. iExists _.
+  iFrame. iPureIntro; split_and!; eauto.
+Qed.
+
+End Laws.
